\section{1 DOF mechanism model}
\begin{equation*}
  \dot{\mtx{x}} = \mtx{A}\mtx{x} + \mtx{B}\mtx{u}
\end{equation*}
\begin{equation*}
  \begin{array}{ccc}
    \mtx{x} = velocity & \dot{\mtx{x}} = acceleration & \mtx{u} = voltage
  \end{array}
\end{equation*}

If $\mtx{u} = K_v v$, then $\mtx{x} = v$ and $\dot{\mtx{x}} = \mtx{0}$.
Therefore
\begin{equation}
  0 = \mtx{A}v + \mtx{B}(K_v v) \label{eq:sysid-eq1}
\end{equation}

If $\mtx{u} = K_v v + K_a a$, then $\mtx{x} = v$ and $\dot{\mtx{x}} = a$.
Therefore
\begin{equation}
  a = \mtx{A}v + \mtx{B}(K_v v + K_a a) \label{eq:sysid-eq2}
\end{equation}

Subtract equation \eqref{eq:sysid-eq1} from equation \eqref{eq:sysid-eq2}.
\begin{align*}
  a &= \mtx{B} (K_a a) \\
  1 &= \mtx{B} K_a \\
  \mtx{B} &= \frac{1}{K_a}
\end{align*}

Substitute $\mtx{B}$ back into \eqref{eq:sysid-eq1} to obtain $\mtx{A}$.
\begin{align*}
  \mtx{0} &= \mtx{A}v + \left(\frac{1}{K_a}\right)(K_v v) \\
  \mtx{0} &= \mtx{A}v + \frac{K_v}{K_a} v \\
  -\frac{K_v}{K_a} v &= \mtx{A}v \\
  \mtx{A} &= -\frac{K_v}{K_a}
\end{align*}

A model with position and velocity states would be
\begin{theorem}[1 DOF mechanism position model]
  \begin{equation*}
    \dot{\mtx{x}} = \mtx{A}\mtx{x} + \mtx{B}\mtx{u}
  \end{equation*}
  \begin{equation*}
    \begin{array}{cc}
    \mtx{x} =
      \begin{bmatrix}
        \text{position} \\
        \text{velocity}
      \end{bmatrix} &
    \mtx{u} =
      \begin{bmatrix}
        \text{voltage}
      \end{bmatrix}
    \end{array}
  \end{equation*}
  \begin{equation}
    \dot{\mtx{x}} =
      \begin{bmatrix}
        0 & 1 \\
        0 & -\frac{K_v}{K_a}
      \end{bmatrix}
      \mtx{x} +
      \begin{bmatrix}
        0 \\
        \frac{1}{K_a}
      \end{bmatrix}
      \mtx{u}
  \end{equation}
\end{theorem}
